Remove references to C.exit_sucess (deprecated)

code/poly1305/Hacl.Test.Poly1305_64.fst
@@ -9,7 +9,7 @@ open Hacl.Cast
 
 module Poly = Poly1305_64
 
-val main: unit -> ST FStar.Int32.t
+val main: unit -> ST C.exit_code
   (requires (fun h -> True))
   (ensures  (fun h0 r h1 -> True))
 let main () =
@@ -40,4 +40,4 @@ let main () =
   Poly.crypto_onetimeauth mac plaintext len' key;
   TestLib.compare_and_print (C.String.of_literal "poly1305") expected mac macsize;
   pop_frame();
-  C.exit_success
+  C.EXIT_SUCCESS
