code/hash/Hacl.Test.SHA2_256.fst
@@ -447,7 +447,7 @@ let test_6 () =
 
 
 
-val main: unit -> ST FStar.Int32.t
+val main: unit -> ST C.exit_code
   (requires (fun h -> True))
   (ensures  (fun h0 r h1 -> True))
 let main () =
@@ -475,4 +475,4 @@ let main () =
   test_6();
 
   (* Exit the program *)
-  C.exit_success
+  C.EXIT_SUCCESS
